Refactored GCM code

AES.v
@@ -1,140 +1,17 @@
+(* AES with 128-bit key *)
+
 Set Implicit Arguments.
 
 Require Import FPUtil.
-
-(* AES with 128-bit key *)
-
 Require Import Arith NArith NPeano Ascii String List.
 Import ListNotations.
-Open Scope N_scope.
-Open Scope nat_scope.
-Open Scope string_scope.
-Open Scope list_scope.
-
-Definition bitvec := list bool.
-
-Definition b128 := bitvec.
-
-Definition b352 := bitvec.
-
-Definition b32 := bitvec.
-
-Definition byte := bitvec.
-
-Definition get_slice A (vec : list A) begin len := firstn len (skipn begin vec).
-
-Definition get (width : nat) (vec : bitvec) (idx : nat) := get_slice vec (width * idx) width.
-
-Definition set_slice A (vec : list A) begin value := firstn begin vec ++ value ++ skipn (begin + length value) vec.
-
-Definition set (width : nat) (vec : bitvec) (idx : nat) value := set_slice vec (width * idx) value.
-
-Definition key_t := b128.
-
-Definition key_schedule_t := b352.
-
-Definition zeros := repeat false.
-
-Definition of_bin_ascii (ch : ascii) :=
-  (match ch with
-     | "0" => false
-     | _ => true
-   end)%char.
-
-Definition bitvec_of_bin_str : string -> bitvec := map of_bin_ascii << str_to_list.
-Coercion bitvec_of_bin_str : string >-> bitvec.
-Notation bin := bitvec_of_bin_str.
-
-Notation t := true.
-Notation f := false.
-
-(* trunc or padding zeros on the right *)
-Definition right_trunc_pad_to len (vec : bitvec) : bitvec := firstn len vec ++ zeros (len - length vec).
-
-(* convert positive to LSB-first bitvec *)
-Fixpoint lsb_of_pos (p : positive) : bitvec :=
-  match p with
-    | xH => [true]
-    | xI p => true :: lsb_of_pos p
-    | xO p => false :: lsb_of_pos p
-  end.
-
-Definition lsb_of_N (n : N) : byte := 
-  match n with
-    | N0 => [false]
-    | Npos p => lsb_of_pos p
-  end.
-
-Fixpoint lsb_to_N (vec : bitvec) : N :=
-  match vec with
-    | nil => N0
-    | b :: vec =>
-      match lsb_to_N vec with
-        | N0 => if b then Npos xH else N0
-        | Npos p => 
-          let p := if b then xI p else xO p in 
-          Npos p
-      end
-  end.
-
-Definition lsb_to_nat : bitvec -> nat := lsb_to_N >> nat_of_N.
-
-Goal lsb_to_nat "1100" = 3. r. Qed.
-Goal lsb_to_nat "1101" = 11. r. Qed.
-
-(* byte is in MSB-first format *)
-
-Arguments rev {A} _.
-
-Definition msb_to_N := rev >> lsb_to_N.
-Definition msb_to_nat := rev >> lsb_to_nat.
-
-(* convert N to MSB-first bitvec *)
-Definition msb_of_N (width : nat) (n : N) : bitvec := 
-  rev $ right_trunc_pad_to width (lsb_of_N n).
-
-Definition msb_of_nat (width : nat) (n : nat) : bitvec := msb_of_N width (N.of_nat n).
-
-Definition byte_of_N (n : N) : byte := msb_of_N 8 n.
-
-Definition byte_of_nat (n : nat) : byte := msb_of_nat 8 n.
-Coercion byte_of_nat : nat >-> byte.
-
-Goal byte_of_nat 3 = "00000011" :> bitvec. r. Qed.
-
-Definition byte_to_nat (b : byte) : nat := msb_to_nat b.
-
-Definition N_of_hex_ascii (ch : ascii) : N := default 0%N $ msum $ map (fun x : ascii * ascii * N => let (p, base) := x in N_of_ascii_in (fst p) (snd p) base ch) [("0", "9", 0%N); ("A", "F", 10%N); ("a", "f", 10%N)]%char.
-
-Definition map_byte (f : byte -> byte) (vec : bitvec) : bitvec := map_every 8 f vec.
-
-(* hex string is in bytewise-MSB-first format *)
-Definition halfbyte_of_hex_ascii := rev << right_trunc_pad_to 4 << lsb_of_N << N_of_hex_ascii.
-
-Definition remove_space (ch : ascii) :=
-  match ch with
-    | " "%char => false
-    | _ => true
-  end.
-
-Definition bitvec_of_hex : string -> bitvec := flat << map halfbyte_of_hex_ascii << filter remove_space << str_to_list.
-
-Definition left_trunc_pad_to n := rev << right_trunc_pad_to n << rev.
-
-Definition byte_of_hex : string -> byte := left_trunc_pad_to 8 << bitvec_of_hex.
-
-Definition halfbyte_to_hex (v : bitvec) : ascii :=
-  let n := lsb_to_nat (rev v) in
-  let n0 := nat_of_ascii "0" in
-  let nA := nat_of_ascii "A" in
-  if n <? 10 then
-    ascii_of_nat (n0 + n)
-  else
-    ascii_of_nat (nA + n - 10).
-
-Goal halfbyte_to_hex "1011" = "B"%char. r. Qed.
-
-Definition bitvec_to_hex := list_to_str << map halfbyte_to_hex << slice 4.
+Local Open Scope prog_scope.
+Local Open Scope N_scope.
+Local Open Scope nat_scope.
+Local Open Scope string_scope.
+Local Open Scope list_scope.
+Require Import Bitvec.
+Local Open Scope bitvec_scope.
 
 Definition s_box : list byte := map byte_of_hex
 [
@@ -190,9 +67,6 @@ Definition list_get (ls : list byte) idx := nth idx ls 0.
 
 Definition sub_byte (b : byte) := list_get s_box (byte_to_nat b).
 
-Notation hex := bitvec_of_hex.
-Notation show := bitvec_to_hex.
-
 Goal (map_byte sub_byte $ hex "cf4f3c09") = hex "8a84eb01". r. Qed.
 
 Definition get_byte := get 8.
@@ -201,18 +75,6 @@ Definition set_byte := set 8.
 Definition lcshift_byte := @lcshift bool 8.
 
 Goal (lcshift_byte $ hex "09cf4f3c") = hex "cf4f3c09". r. Qed.
-
-Definition bit_xor (a b : bool) : bool :=
-  match a, b with
-    | true, false => true
-    | false, true => true
-    | _, _ => false
-  end.
-
-Definition xor (a b : bitvec) : bitvec := map2 bit_xor a b.
-
-Infix "+" := xor : bitvec_scope.
-Open Scope bitvec_scope.
 
 Definition g n (w : key_t) :=
   let w := lcshift_byte w in
@@ -290,27 +152,6 @@ Definition inv_mix_matrix : matrix byte := to_row_major_mx 4 4 $ slice 8 $ flat 
   "0d 09 0e 0b";
   "0b 0d 09 0e"
 ].
-
-Definition f231 A B C D (f : A -> B -> C -> D) b c a := f a b c.
-
-Definition rshift n (v : bitvec) := zeros n ++ firstn (length v - n) v.
-
-Arguments fst {A B} _.
-Arguments fold_left {A B} _ _ _.
-
-Definition gf_mul n R (a b : bitvec) : bitvec :=
-  let R := right_trunc_pad_to n R in
-  fst $ f231 fold_left b (zeros n, a) (fun st bi =>
-    let (Z, V) := st in
-    let Z := if bi then
-               Z + V
-             else
-               Z in
-    let V := if nth (n - 1) V false then
-               rshift 1 V + R
-             else
-               rshift 1 V in
-    (Z, V)).
 
 Definition gf8_byte_mul (a b : byte) : byte := rev $ gf_mul 8 "11011" (rev a) (rev b).
 
