Bitvec.v
@@ -1,0 +1,182 @@
+(* bit vectors. Not length-indexed *)
+
+Set Implicit Arguments.
+
+Require Import FPUtil.
+
+Require Import Arith NArith NPeano Ascii String List.
+Import ListNotations.
+Local Open Scope prog_scope.
+Local Open Scope N_scope.
+Local Open Scope nat_scope.
+Local Open Scope string_scope.
+Local Open Scope list_scope.
+
+Definition bitvec := list bool.
+
+Definition b128 := bitvec.
+
+Definition b352 := bitvec.
+
+Definition b32 := bitvec.
+
+Definition byte := bitvec.
+
+Definition get_slice A (vec : list A) begin len := firstn len (skipn begin vec).
+
+Definition get (width : nat) (vec : bitvec) (idx : nat) := get_slice vec (width * idx) width.
+
+Definition set_slice A (vec : list A) begin value := firstn begin vec ++ value ++ skipn (begin + length value) vec.
+
+Definition set (width : nat) (vec : bitvec) (idx : nat) value := set_slice vec (width * idx) value.
+
+Definition key_t := b128.
+
+Definition key_schedule_t := b352.
+
+Definition zeros := repeat false.
+
+Definition of_bin_ascii (ch : ascii) :=
+  (match ch with
+     | "0" => false
+     | _ => true
+   end)%char.
+
+Definition bitvec_of_bin_str : string -> bitvec := map of_bin_ascii << str_to_list.
+Coercion bitvec_of_bin_str : string >-> bitvec.
+Notation bin := bitvec_of_bin_str.
+
+Notation t := true.
+Notation f := false.
+
+(* trunc or padding zeros on the right *)
+Definition right_trunc_pad_to len (vec : bitvec) : bitvec := firstn len vec ++ zeros (len - length vec).
+
+(* convert positive to LSB-first bitvec *)
+Fixpoint lsb_of_pos (p : positive) : bitvec :=
+  match p with
+    | xH => [true]
+    | xI p => true :: lsb_of_pos p
+    | xO p => false :: lsb_of_pos p
+  end.
+
+Definition lsb_of_N (n : N) : byte := 
+  match n with
+    | N0 => [false]
+    | Npos p => lsb_of_pos p
+  end.
+
+Fixpoint lsb_to_N (vec : bitvec) : N :=
+  match vec with
+    | nil => N0
+    | b :: vec =>
+      match lsb_to_N vec with
+        | N0 => if b then Npos xH else N0
+        | Npos p => 
+          let p := if b then xI p else xO p in 
+          Npos p
+      end
+  end.
+
+Definition lsb_to_nat : bitvec -> nat := lsb_to_N >> nat_of_N.
+
+Goal lsb_to_nat "1100" = 3. r. Qed.
+Goal lsb_to_nat "1101" = 11. r. Qed.
+
+(* byte is in MSB-first format *)
+
+Arguments rev {A} _.
+
+Definition msb_to_N := rev >> lsb_to_N.
+Definition msb_to_nat := rev >> lsb_to_nat.
+
+(* convert N to MSB-first bitvec *)
+Definition msb_of_N (width : nat) (n : N) : bitvec := 
+  rev $ right_trunc_pad_to width (lsb_of_N n).
+
+Definition msb_of_nat (width : nat) (n : nat) : bitvec := msb_of_N width (N.of_nat n).
+
+Definition byte_of_N (n : N) : byte := msb_of_N 8 n.
+
+Definition byte_of_nat (n : nat) : byte := msb_of_nat 8 n.
+Coercion byte_of_nat : nat >-> byte.
+
+Goal byte_of_nat 3 = "00000011" :> bitvec. r. Qed.
+
+Definition byte_to_nat (b : byte) : nat := msb_to_nat b.
+
+Definition N_of_hex_ascii (ch : ascii) : N := default 0%N $ msum $ map (fun x : ascii * ascii * N => let (p, base) := x in N_of_ascii_in (fst p) (snd p) base ch) [("0", "9", 0%N); ("A", "F", 10%N); ("a", "f", 10%N)]%char.
+
+Definition map_byte (f : byte -> byte) (vec : bitvec) : bitvec := map_every 8 f vec.
+
+(* hex string is in bytewise-MSB-first format *)
+Definition halfbyte_of_hex_ascii := rev << right_trunc_pad_to 4 << lsb_of_N << N_of_hex_ascii.
+
+Definition remove_space (ch : ascii) :=
+  match ch with
+    | " "%char => false
+    | _ => true
+  end.
+
+Definition bitvec_of_hex : string -> bitvec := flat << map halfbyte_of_hex_ascii << filter remove_space << str_to_list.
+
+Definition left_trunc_pad_to n := rev << right_trunc_pad_to n << rev.
+
+Definition byte_of_hex : string -> byte := left_trunc_pad_to 8 << bitvec_of_hex.
+
+Definition halfbyte_to_hex (v : bitvec) : ascii :=
+  let n := lsb_to_nat (rev v) in
+  let n0 := nat_of_ascii "0" in
+  let nA := nat_of_ascii "A" in
+  if n <? 10 then
+    ascii_of_nat (n0 + n)
+  else
+    ascii_of_nat (nA + n - 10).
+
+Goal halfbyte_to_hex "1011" = "B"%char. r. Qed.
+
+Definition bitvec_to_hex := list_to_str << map halfbyte_to_hex << slice 4.
+
+Notation hex := bitvec_of_hex.
+Notation show := bitvec_to_hex.
+
+Definition bitvec_eqb := forall2 Bool.eqb.
+Infix "=?" := bitvec_eqb : bitvec_scope.
+Local Open Scope bitvec_scope.
+
+Goal bin "101" =? bin "101" = true. r. Qed.
+Goal bin "101" =? bin "10" = false. r. Qed.
+Goal hex "ab" =? hex "ab" = true. r. Qed.
+Goal hex "ab" =? hex "ac" = false. r. Qed.
+
+Definition bit_xor (a b : bool) : bool :=
+  match a, b with
+    | true, false => true
+    | false, true => true
+    | _, _ => false
+  end.
+
+Definition xor (a b : bitvec) : bitvec := map2 bit_xor a b.
+
+Definition rshift n (v : bitvec) := zeros n ++ firstn (length v - n) v.
+
+Arguments fst {A B} _.
+Arguments fold_left {A B} _ _ _.
+
+Definition f231 A B C D (f : A -> B -> C -> D) b c a := f a b c.
+
+Infix "+" := xor : bitvec_scope.
+
+Definition gf_mul n R (a b : bitvec) : bitvec :=
+  let R := right_trunc_pad_to n R in
+  fst $ f231 fold_left b (zeros n, a) (fun st bi =>
+    let (Z, V) := st in
+    let Z := if bi then
+               Z + V
+             else
+               Z in
+    let V := if nth (n - 1) V false then
+               rshift 1 V + R
+             else
+               rshift 1 V in
+    (Z, V)).
