GCMTest.v
@@ -1,0 +1,197 @@
+Set Implicit Arguments.
+
+Require Import FPUtil.
+
+Require Import Arith NArith NPeano Ascii String List Bool.
+Import ListNotations.
+Local Open Scope prog_scope.
+Local Open Scope N_scope.
+Local Open Scope nat_scope.
+Local Open Scope string_scope.
+Local Open Scope list_scope.
+Local Open Scope bool_scope.
+Require Import Bitvec.
+Local Open Scope bitvec_scope.
+
+Require Import GCM.
+
+Require AES.
+Notation E := AES.encrypt.
+
+Module test1.
+  Definition t_K := hex "00000000000000000000000000000000".
+  Definition t_P := hex "".
+  Definition t_IV := hex "000000000000000000000000".
+  Definition t_H := hex "66e94bd4ef8a2c3b884cfa59ca342b2e".
+  Goal (H E t_K) = t_H. r. Qed.
+  Definition t_Y0 := hex "00000000000000000000000000000001".
+  Goal (Y0 E t_K t_IV) = t_Y0. r. Qed.
+  Definition t_E_K_Y0 := hex "58e2fccefa7e3061367f1d57a4e7455a".
+  Goal E t_K t_Y0 = t_E_K_Y0. r. Qed.
+  Definition t_C := hex "".
+  Goal (Encrypt E t_K t_IV t_P) = t_C. r. Qed.
+  Definition t_lenA_lenC := hex "00000000000000000000000000000000".
+  Definition t_A := hex "".
+  Goal len t_A ++ len t_C = t_lenA_lenC. r. Qed.
+  Definition t_GHASH := hex "00000000000000000000000000000000".
+  Goal GHASH t_H t_A t_C = t_GHASH. r. Qed.
+  Definition t_T := hex "58e2fccefa7e3061367f1d57a4e7455a".
+  Definition t_t := 128.
+  Goal encrypt E t_K t_IV t_P t_A t_t = (t_C, t_T). r. Qed.
+  Goal (decrypt E t_K t_IV t_C t_A t_T) = Some t_P. r. Qed.
+End test1.
+
+Module test2.
+  Definition t_K := hex "00000000000000000000000000000000".
+  Definition t_P := hex "00000000000000000000000000000000".
+  Definition t_IV := hex "000000000000000000000000".
+  Definition t_H := hex "66e94bd4ef8a2c3b884cfa59ca342b2e".
+  Goal (H E t_K) = t_H. r. Qed.
+  Definition t_Y0 := hex "00000000000000000000000000000001".
+  Goal (Y0 E t_K t_IV) = t_Y0. r. Qed.
+  Definition t_E_K_Y0 := hex "58e2fccefa7e3061367f1d57a4e7455a".
+  Goal E t_K t_Y0 = t_E_K_Y0. r. Qed.
+  Definition t_C := hex "0388dace60b6a392f328c2b971b2fe78".
+  Goal (Encrypt E t_K t_IV t_P) = t_C. r. Qed.
+  Definition t_lenA_lenC := hex "00000000000000000000000000000080".
+  Definition t_A := hex "".
+  Goal len t_A ++ len t_C = t_lenA_lenC. r. Qed.
+  Definition t_GHASH := hex "f38cbb1ad69223dcc3457ae5b6b0f885".
+  Goal GHASH t_H t_A t_C = t_GHASH. r. Qed.
+  Definition t_T := hex "ab6e47d42cec13bdf53a67b21257bddf".
+  Definition t_t := 128.
+  Goal encrypt E t_K t_IV t_P t_A t_t = (t_C, t_T). r. Qed.
+  Goal (decrypt E t_K t_IV t_C t_A t_T) = Some t_P. r. Qed.
+  Definition noise := left_trunc_pad_to (length t_C) $ hex "000001000".
+  Goal (decrypt E t_K t_IV (t_C + noise) t_A t_T) = None. r. Qed.
+End test2.
+
+Module test3.
+  Definition t_K := hex "feffe9928665731c6d6a8f9467308308".
+  Definition t_P := flat $ map hex ["d9313225f88406e5a55909c5aff5269a";
+                                     "86a7a9531534f7da2e4c303d8a318a72";
+                                     "1c3c0c95956809532fcf0e2449a6b525";
+                                     "b16aedf5aa0de657ba637b391aafd255"].
+  Definition t_IV := hex "cafebabefacedbaddecaf888".
+  Definition t_H := hex "b83b533708bf535d0aa6e52980d53b78".
+  Goal (H E t_K) = t_H. r. Qed.
+  Definition t_Y0 := hex "cafebabefacedbaddecaf88800000001".
+  Goal (Y0 E t_K t_IV) = t_Y0. r. Qed.
+  Definition t_E_K_Y0 := hex "3247184b3c4f69a44dbcd22887bbb418".
+  Goal E t_K t_Y0 = t_E_K_Y0. r. Qed.
+  Definition t_C := flat $ map hex ["42831ec2217774244b7221b784d0d49c";
+                                     "e3aa212f2c02a4e035c17e2329aca12e";
+                                     "21d514b25466931c7d8f6a5aac84aa05";
+                                     "1ba30b396a0aac973d58e091473f5985"].
+  Goal (Encrypt E t_K t_IV t_P) = t_C. r. Qed.
+  Definition t_lenA_lenC := hex "00000000000000000000000000000200".
+  Definition t_A := hex "".
+  Goal len t_A ++ len t_C = t_lenA_lenC. r. Qed.
+  Definition t_GHASH := hex "7f1b32b81b820d02614f8895ac1d4eac".
+  Goal GHASH t_H t_A t_C = t_GHASH. r. Qed.
+  Definition t_T := hex "4d5c2af327cd64a62cf35abd2ba6fab4".
+  Definition t_t := 128.
+  Goal encrypt E t_K t_IV t_P t_A t_t = (t_C, t_T). r. Qed.
+  Goal (decrypt E t_K t_IV t_C t_A t_T) = Some t_P. r. Qed.
+  Definition noise := left_trunc_pad_to (length t_C) $ hex "000001000".
+  Goal (decrypt E t_K t_IV (t_C + noise) t_A t_T) = None. r. Qed.
+End test3.
+
+Module test4.
+  Definition t_K := hex "feffe9928665731c6d6a8f9467308308".
+  Definition t_P := flat $ map hex ["d9313225f88406e5a55909c5aff5269a";
+                                     "86a7a9531534f7da2e4c303d8a318a72";
+                                     "1c3c0c95956809532fcf0e2449a6b525";
+                                     "b16aedf5aa0de657ba637b39"].
+  Definition t_A := flat $ map hex ["feedfacedeadbeeffeedfacedeadbeef";
+                                     "abaddad2"].
+  Definition t_IV := hex "cafebabefacedbaddecaf888".
+  Definition t_H := hex "b83b533708bf535d0aa6e52980d53b78".
+  Goal (H E t_K) = t_H. r. Qed.
+  Definition t_Y0 := hex "cafebabefacedbaddecaf88800000001".
+  Goal (Y0 E t_K t_IV) = t_Y0. r. Qed.
+  Definition t_E_K_Y0 := hex "3247184b3c4f69a44dbcd22887bbb418".
+  Goal E t_K t_Y0 = t_E_K_Y0. r. Qed.
+  Definition t_C := flat $ map hex ["42831ec2217774244b7221b784d0d49c";
+                                     "e3aa212f2c02a4e035c17e2329aca12e";
+                                     "21d514b25466931c7d8f6a5aac84aa05";
+                                     "1ba30b396a0aac973d58e091"].
+  Goal (Encrypt E t_K t_IV t_P) = t_C. r. Qed.
+  Definition t_lenA_lenC := hex "00000000000000a000000000000001e0".
+  Goal len t_A ++ len t_C = t_lenA_lenC. r. Qed.
+  Definition t_GHASH := hex "698e57f70e6ecc7fd9463b7260a9ae5f".
+  Goal GHASH t_H t_A t_C = t_GHASH. r. Qed.
+  Definition t_T := hex "5bc94fbc3221a5db94fae95ae7121a47".
+  Definition t_t := 128.
+  Goal encrypt E t_K t_IV t_P t_A t_t = (t_C, t_T). r. Qed.
+  Goal (decrypt E t_K t_IV t_C t_A t_T) = Some t_P. r. Qed.
+  Definition noise := left_trunc_pad_to (length t_C) $ hex "000001000".
+  Goal (decrypt E t_K t_IV (t_C + noise) t_A t_T) = None. r. Qed.
+End test4.
+
+Module test5.
+  Definition t_K := hex "feffe9928665731c6d6a8f9467308308".
+  Definition t_P := flat $ map hex ["d9313225f88406e5a55909c5aff5269a";
+                                     "86a7a9531534f7da2e4c303d8a318a72";
+                                     "1c3c0c95956809532fcf0e2449a6b525";
+                                     "b16aedf5aa0de657ba637b39"].
+  Definition t_A := flat $ map hex ["feedfacedeadbeeffeedfacedeadbeef";
+                                     "abaddad2"].
+  Definition t_IV := hex "cafebabefacedbad".
+  Definition t_H := hex "b83b533708bf535d0aa6e52980d53b78".
+  Goal (H E t_K) = t_H. r. Qed.
+  Definition t_Y0 := hex "c43a83c4c4badec4354ca984db252f7d".
+  Goal (Y0 E t_K t_IV) = t_Y0. r. Qed.
+  Definition t_E_K_Y0 := hex "e94ab9535c72bea9e089c93d48e62fb0".
+  Goal E t_K t_Y0 = t_E_K_Y0. r. Qed.
+  Definition t_C := flat $ map hex ["61353b4c2806934a777ff51fa22a4755";
+                                     "699b2a714fcdc6f83766e5f97b6c7423";
+                                     "73806900e49f24b22b097544d4896b42";
+                                     "4989b5e1ebac0f07c23f4598"].
+  Goal (Encrypt E t_K t_IV t_P) = t_C. r. Qed.
+  Definition t_lenA_lenC := hex "00000000000000a000000000000001e0".
+  Goal len t_A ++ len t_C = t_lenA_lenC. r. Qed.
+  Definition t_GHASH := hex "df586bb4c249b92cb6922877e444d37b".
+  Goal GHASH t_H t_A t_C = t_GHASH. r. Qed.
+  Definition t_T := hex "3612d2e79e3b0785561be14aaca2fccb".
+  Definition t_t := 128.
+  Goal encrypt E t_K t_IV t_P t_A t_t = (t_C, t_T). r. Qed.
+  Goal (decrypt E t_K t_IV t_C t_A t_T) = Some t_P. r. Qed.
+  Definition noise := left_trunc_pad_to (length t_C) $ hex "000001000".
+  Goal (decrypt E t_K t_IV (t_C + noise) t_A t_T) = None. r. Qed.
+End test5.
+
+Module test6.
+  Definition t_K := hex "feffe9928665731c6d6a8f9467308308".
+  Definition t_P := flat $ map hex ["d9313225f88406e5a55909c5aff5269a";
+                                     "86a7a9531534f7da2e4c303d8a318a72";
+                                     "1c3c0c95956809532fcf0e2449a6b525";
+                                     "b16aedf5aa0de657ba637b39"].
+  Definition t_A := flat $ map hex ["feedfacedeadbeeffeedfacedeadbeef";
+                                     "abaddad2"].
+  Definition t_IV := flat $ map hex ["9313225df88406e555909c5aff5269aa";
+                                      "6a7a9538534f7da1e4c303d2a318a728";
+                                      "c3c0c95156809539fcf0e2429a6b5254";
+                                      "16aedbf5a0de6a57a637b39b"].
+  Definition t_H := hex "b83b533708bf535d0aa6e52980d53b78".
+  Goal (H E t_K) = t_H. r. Qed.
+  Definition t_Y0 := hex "3bab75780a31c059f83d2a44752f9864".
+  Goal (Y0 E t_K t_IV) = t_Y0. r. Qed.
+  Definition t_E_K_Y0 := hex "7dc63b399f2d98d57ab073b6baa4138e".
+  Goal E t_K t_Y0 = t_E_K_Y0. r. Qed.
+  Definition t_C := flat $ map hex ["8ce24998625615b603a033aca13fb894";
+                                     "be9112a5c3a211a8ba262a3cca7e2ca7";
+                                     "01e4a9a4fba43c90ccdcb281d48c7c6f";
+                                     "d62875d2aca417034c34aee5"].
+  Goal (Encrypt E t_K t_IV t_P) = t_C. r. Qed.
+  Definition t_lenA_lenC := hex "00000000000000a000000000000001e0".
+  Goal len t_A ++ len t_C = t_lenA_lenC. r. Qed.
+  Definition t_GHASH := hex "1c5afe9760d3932f3c9a878aac3dc3de".
+  Goal GHASH t_H t_A t_C = t_GHASH. r. Qed.
+  Definition t_T := hex "619cc5aefffe0bfa462af43c1699d050".
+  Definition t_t := 128.
+  Goal encrypt E t_K t_IV t_P t_A t_t = (t_C, t_T). r. Qed.
+  Goal (decrypt E t_K t_IV t_C t_A t_T) = Some t_P. r. Qed.
+  Definition noise := left_trunc_pad_to (length t_C) $ hex "000001000".
+  Goal (decrypt E t_K t_IV (t_C + noise) t_A t_T) = None. r. Qed.
+End test6.
